src/program_proof/mvcc/tuple_kill_version.v
@@ -44,46 +44,26 @@ Proof.
   by rewrite fmap_app.
 Qed.
 
-Definition tuple_killed tuple (tid : u64) (key : u64) γ : iProp Σ :=
-  ∃ (tidown tidlast tidgc : u64) (vers : list pver)
-    (vchain : list dbval),
-    (* physical state is updated, but logical state is not. *)
-    let vers' := vers ++ [(tid, true, (U64 0))] in
-    "Hphys" ∷ own_tuple_phys tuple (U64 0) (U64 (int.Z tid + 1)) vers' ∗
-    "Habst" ∷ own_tuple_abst key tidown tidlast tidgc vers vchain γ ∗
-    "%Htid" ∷ ⌜int.Z tidgc ≤ int.Z tid⌝.
-
 (*****************************************************************)
 (* func (tuple *Tuple) KillVersion(tid uint64) uint64            *)
 (*****************************************************************)
-Theorem wp_tuple__KillVersion tuple (tid : u64) (key : u64) (sid : u64) γ :
-  is_tuple tuple key γ -∗
-  {{{ active_tid γ tid sid }}}
+Theorem wp_tuple__KillVersion
+        tuple (tid : u64) (key : u64) (sid : u64)
+        (phys : list dbval) γ :
+  {{{ active_tid γ tid sid ∗
+      own_tuple_locked tuple key tid phys (extend (S (int.nat tid)) phys ++ [Nil]) γ
+  }}}
     Tuple__KillVersion #tuple #tid
-  {{{ (latch : loc) (ret : u64), RET #ret;
-      active_tid γ tid sid ∗
-      tuple_locked tuple key latch γ ∗
-      tuple_killed tuple tid key γ
-  }}}.
+  {{{ (ret : u64), RET #ret; active_tid γ tid sid }}}.
 Proof.
-  iIntros "#Htuple" (Φ) "!> Hactive HΦ".
-  iNamed "Htuple".
+  iIntros (Φ) "[Hactive H] HΦ".
   wp_call.
-  
-  (***********************************************************)
-  (* tuple.latch.Lock()                                      *)
-  (***********************************************************)
-  wp_loadField.
-  wp_apply (acquire_spec with "Hlock").
-  iIntros "[Hlocked HtupleOwn]".
-  iNamed "HtupleOwn".
-  iNamed "Habst".
 
   (***********************************************************)
   (* ok := tuple.killVersion(tid)                            *)
   (***********************************************************)
-  iNamed "Hphys".
-  wp_apply (wp_tuple__killVersion with "[$Htidown $Htidlast Hvers HversS]"); first eauto with iFrame.
+  iNamed "H".
+  wp_apply (wp_tuple__killVersion with "Hphys").
   iIntros (ok) "Hphys".
   wp_pures.
   
@@ -125,23 +105,119 @@ Proof.
   (***********************************************************)
   (* tuple.rcond.Broadcast()                                 *)
   (***********************************************************)
+  iNamed "Hlock".
   wp_loadField.
   wp_apply (wp_condBroadcast with "[$HrcondC]").
   
-  wp_pures.
-  wp_load.
+  (***********************************************************)
+  (* tuple.latch.Unlock()                                    *)
+  (***********************************************************)
+  iNamed "Hrepr".
+  iApply fupd_wp.
   iInv "Hinvgc" as ">HinvgcO" "HinvgcC".
   iDestruct (active_ge_min with "HinvgcO Hactive Hgclb") as "%HtidGe".
   iMod ("HinvgcC" with "HinvgcO") as "_".
   iModIntro.
-  rewrite ite_apply.
-  iApply "HΦ".
-  iFrame "# ∗".
-  unfold tuple_killed.
-  do 5 iExists _.
-  iFrame "Hphys".
-  iSplit; last done.
-  iFrame "% # ∗".
+  wp_loadField.
+  assert (HlenN : length phys = S (int.nat tidlast)) by word.
+  iAssert (⌜int.Z tid < 2 ^ 64 - 1⌝)%I with "[Hactive]" as "%Htidmax".
+  { iDestruct "Hactive" as "[_ %H]". iPureIntro. word. }
+  wp_apply (release_spec with "[-HΦ Hactive HretR]").
+  { iFrame "Hlock Hlocked".
+    iNext.
+    erewrite extend_last_Some; last apply Hlast.
+    rewrite -app_assoc.
+    set phys' := phys ++ _ ++ _.
+    iExists (U64 0), (U64 (int.Z tid + 1)), tidgc, _, phys'.
+    iFrame "Hphys Hptuple".
+    iNamed "Hwellformed".
+    iSplit.
+    { (* Prove [HtupleAbs]. *)
+      iPureIntro.
+      simpl.
+      intros tidx Htidx.
+      destruct (decide (int.Z tidx ≤ int.Z tidlast)); subst phys'.
+      - (* Reading the non-extension part. *)
+        rewrite lookup_app_l; last word.
+        rewrite HtupleAbs; last word.
+        symmetry.
+        f_equal.
+        apply spec_lookup_snoc_l with tid; [done | word].
+      - (* Reading the extension part. *)
+        rewrite lookup_app_r; last word.
+        apply Znot_le_gt in n.
+        destruct (decide (int.Z tidx ≤ int.Z tid)).
+        + (* Reading the old value. *)
+          rewrite lookup_app_l; last first.
+          { rewrite HlenN replicate_length. word. }
+          rewrite lookup_replicate_2; last word.
+          f_equal.
+          rewrite (spec_lookup_snoc_l _ _ _ tid); [| auto | word].
+          apply spec_lookup_extensible with tidlast; [word | word | auto].
+        + (* Reading the new value. *)
+          apply Znot_le_gt in n0.
+          rewrite lookup_app_r; last first.
+          { rewrite HlenN replicate_length. word. }
+          replace (int.Z (U64 _)) with (int.Z tid + 1) in Htidx by word.
+          assert (Etidx : int.Z tidx = int.Z tid + 1) by word.
+          replace (int.nat tidx - _ - _)%nat with 0%nat; last first.
+          { rewrite replicate_length. word. }
+          simpl. f_equal.
+          rewrite (spec_lookup_snoc_r _ _ _ tid); [done | auto | word].
+    }
+    iSplit.
+    { (* Prove [Hlast]. *)
+      iPureIntro.
+      subst phys'.
+      rewrite app_assoc.
+      rewrite last_snoc.
+      f_equal.
+      rewrite (spec_lookup_snoc_r _ _ _ tid); [done | by simpl | word].
+    }
+    iSplit.
+    { (* Prove [HvchainLen]. *)
+      iPureIntro.
+      subst phys'.
+      do 2 rewrite app_length.
+      rewrite HlenN replicate_length singleton_length. word.
+    }
+    iSplit; first done.
+    { (* Prove [Hwellformed]. *)
+      iPureIntro.
+      split.
+      { (* Prove [HtidlastGe]. *)
+        apply Forall_app_2.
+        - apply (Forall_impl _ _ _ HtidlastGt).
+          intros verx Hverx.
+          trans (int.Z tid); word.
+        - rewrite Forall_singleton. simpl. word.
+      }
+      split.
+      { (* Prove [HexistsLt]. *)
+        intros tidx HtidxGZ Htidx.
+        apply Exists_app.
+        left.
+        apply HexistsLt; done.
+      }
+      split.
+      { (* Prove [HtidgcLe]. *)
+        destruct vers eqn:Evers; first contradiction.
+        simpl.
+        apply Forall_app_2; first done.
+        by apply Forall_singleton.
+      }
+      { (* Prove [Hnotnil]. *)
+        apply not_eq_sym.
+        apply app_cons_not_nil.
+      }
+    }
+  }
+
+  (* Return. *)
+  wp_pures.
+  do 2 rewrite ite_apply.
+  wp_load.
+  by iApply "HΦ".
 Qed.
 
 End proof.
