src/program_proof/mvcc/tuple_proof.v
@@ -1,3 +1,3 @@
 From Perennial.program_proof.mvcc Require Export
      tuple_common tuple_append_version tuple_kill_version tuple_read_version
-     tuple_remove_versions tuple_own tuple_free tuple_release.
+     tuple_remove_versions tuple_own tuple_free tuple_write_lock.
