src/program_proof/mvcc/tuple_write_lock.v
@@ -1,0 +1,50 @@
+From Perennial.program_proof.mvcc Require Import tuple_common.
+
+Section proof.
+Context `{!heapGS Σ, !mvcc_ghostG Σ}.
+
+(*****************************************************************)
+(* func (tuple *Tuple) WriteLock()                               *)
+(*****************************************************************)
+Theorem wp_tuple__WriteLock tuple (tid : u64) (key : u64) γ :
+  is_tuple tuple key γ -∗
+  {{{ mods_token γ key (int.nat tid) }}}
+    Tuple__WriteLock #tuple
+  {{{ (phys : list dbval), RET #(); own_tuple_locked tuple key tid phys phys γ }}}.
+Proof.
+  iIntros "#Htuple" (Φ) "!> Htoken HΦ".
+  wp_call.
+  
+  (***********************************************************)
+  (* tuple.latch.Lock()                                      *)
+  (***********************************************************)
+  iNamed "Htuple".
+  wp_loadField.
+  wp_apply (acquire_spec with "Hlock").
+  iIntros "[Hlocked HtupleOwn]".
+  wp_pures.
+
+  iNamed "HtupleOwn".
+  iDestruct "Htoken" as (phys) "[Hptuple' %Hlen]".
+  destruct (decide (tidown = 0)).
+  { (* Obtain contradiction for case [tidown = 0]. *)
+    iInv "Hinv" as "> HinvO" "HinvC".
+    iNamed "HinvO".
+    iDestruct (big_sepS_elem_of _ _ key with "Hkeys") as "Hkey"; first set_solver.
+    iRename "Hptuple" into "Hptuple''".
+    iNamed "Hkey".
+    iDestruct (vchain_combine with "Hptuple Hptuple'") as "[Hptuple _]"; first done.
+    iDestruct (vchain_combine with "Hptuple Hptuple''") as "[Hptuple _]"; first done.
+    iDestruct (vchain_false with "Hptuple") as "contra"; done.
+  }
+  
+  iDestruct (vchain_combine with "Hptuple Hptuple'") as "[Hptuple <-]"; first done.
+  rewrite Qp_quarter_quarter.
+  iModIntro.
+  iApply "HΦ".
+  do 4 iExists _.
+  iFrame "Hptuple Hphys Hrepr".
+  iSplit; [by eauto 10 with iFrame | done].
+Qed.
+
+End proof.
