src/program_proof/mvcc/txn_apply.v
@@ -6,7 +6,7 @@ Context `{!heapGS Σ, !mvcc_ghostG Σ}.
 Theorem wp_txn__apply txn tid view γ τ :
   {{{ own_txn_ready txn tid view γ τ }}}
     Txn__apply #txn
-  {{{ RET #(); own_txn_applied txn tid view γ τ }}}.
+  {{{ RET #(); own_txn txn tid view γ τ }}}.
 Proof.
   (***********************************************************)
   (* ents := txn.wrbuf.IntoEnts()                            *)
